@prefix : <http://www.semanticweb.org/djem/ontologies/2024/9/DogSportConnect/> .
@prefix owl: <http://www.w3.org/2002/07/owl#> .
@prefix rdf: <http://www.w3.org/1999/02/22-rdf-syntax-ns#> .
@prefix xml: <http://www.w3.org/XML/1998/namespace> .
@prefix xsd: <http://www.w3.org/2001/XMLSchema#> .
@prefix rdfs: <http://www.w3.org/2000/01/rdf-schema#> .
@base <http://www.semanticweb.org/djem/ontologies/2024/9/DogSportConnect/> .

<http://www.semanticweb.org/djem/ontologies/2024/9/DogSportConnect> rdf:type owl:Ontology ;
                                                                     rdfs:comment "The ontology will describe dog sports activities and social interactions, including venues, sports types, events, and relationships between owners." ;
                                                                     rdfs:label "The \"Dod Sport Connect\" ontology" .

#################################################################
#    Object Properties
#################################################################

###  http://www.semanticweb.org/djem/ontologies/2024/9/DogSportConnect#cooperatesWith
:cooperatesWith rdf:type owl:ObjectProperty ,
                         owl:SymmetricProperty ;
                rdfs:domain :Owner ;
                rdfs:range :Trainer ;
                rdfs:comment "Indicates that the owner works with a specific trainer" ;
                rdfs:label "cooperatesWith" .


###  http://www.semanticweb.org/djem/ontologies/2024/9/DogSportConnect#ownerAttends
:ownerAttends rdf:type owl:ObjectProperty ;
              owl:propertyChainAxiom ( :attends
                                     ) ,
                                     ( :hasOwner
                                     ) ;
              rdfs:comment "Indicats that owner attends the event" ;
              rdfs:label "ownerAttends" .


###  http://www.semanticweb.org/djem/ontologies/2024/9/DogSportConnect#ownerParticipatesIn
:ownerParticipatesIn rdf:type owl:ObjectProperty ;
                     owl:propertyChainAxiom ( :hasOwner
                                            ) ,
                                            ( :participatesIn
                                            ) ;
                     rdfs:comment "Indicates that owner participates in the specific sport activity with his Dog" ;
                     rdfs:label "ownerParticipatesIn" .


###  http://www.semanticweb.org/djem/ontologies/2024/9/DogSportConnect#ownerTrainedBy
:ownerTrainedBy rdf:type owl:ObjectProperty ;
                owl:propertyChainAxiom ( :hasOwner
                                       ) ,
                                       ( :isTrainedBy
                                       ) ;
                rdfs:comment "Indicates that the owner is trained along with his dog in specific skills by a specific trainer." ;
                rdfs:label "ownerTrainedBy" .


###  http://www.semanticweb.org/djem/ontologies/2024/9/DogSportConnect#ownerTrainsAt
:ownerTrainsAt rdf:type owl:ObjectProperty ;
               owl:propertyChainAxiom ( :hasOwner
                                      ) ,
                                      ( :trainsAt
                                      ) ;
               rdfs:comment "Indicates that the owner along with his Dog trains at specific Venue" ;
               rdfs:label "ownerTrainsAt" .


###  http://www.semanticweb.org/djem/ontologies/2024/9/DogSportConnect/attends
:attends rdf:type owl:ObjectProperty ,
                  owl:AsymmetricProperty ,
                  owl:IrreflexiveProperty ;
         rdfs:domain :Dog ;
         rdfs:range :Event ;
         rdfs:comment "Indicates that an individual participates in an event or a training session." ;
         rdfs:label "dogAttends" .


###  http://www.semanticweb.org/djem/ontologies/2024/9/DogSportConnect/hasInterestIn
:hasInterestIn rdf:type owl:ObjectProperty ;
               rdfs:domain :Owner ;
               rdfs:range :Sports_Activity ;
               rdfs:comment "Represents the interest of an individual in a specific sport or activity." ;
               rdfs:label "hasInterestIn" .


###  http://www.semanticweb.org/djem/ontologies/2024/9/DogSportConnect/hasOwner
:hasOwner rdf:type owl:ObjectProperty ,
                   owl:AsymmetricProperty ;
          rdfs:domain :Dog ;
          rdfs:range :Owner ;
          rdfs:comment "Indicates the ownership relation between a dog and its owner." ;
          rdfs:label "hasOwner" .


###  http://www.semanticweb.org/djem/ontologies/2024/9/DogSportConnect/hosts
:hosts rdf:type owl:ObjectProperty ;
       rdfs:domain :Training_venue ;
       rdfs:range :Event ;
       rdfs:comment "Represents an entity hosting a specific event or activity." ;
       rdfs:label "hosts" .


###  http://www.semanticweb.org/djem/ontologies/2024/9/DogSportConnect/isAlsoTrainer
:isAlsoTrainer rdf:type owl:ObjectProperty ,
                        owl:SymmetricProperty ;
               rdfs:domain :Owner ;
               rdfs:range :Trainer ;
               rdfs:comment "Indicates that an individual also serves as a trainer, aside from their primary role." ;
               rdfs:label "isAlsoTrainer" .


###  http://www.semanticweb.org/djem/ontologies/2024/9/DogSportConnect/isPartOf
:isPartOf rdf:type owl:ObjectProperty ,
                   owl:FunctionalProperty ,
                   owl:AsymmetricProperty ,
                   owl:IrreflexiveProperty ;
          rdfs:domain :Event ;
          rdfs:range :Sports_Activity ;
          rdfs:comment "Shows that an entity is a part of a larger event or group." ;
          rdfs:label "isPartOf" .


###  http://www.semanticweb.org/djem/ontologies/2024/9/DogSportConnect/isSuitableForActivity
:isSuitableForActivity rdf:type owl:ObjectProperty ;
                       rdfs:domain :Dog ;
                       rdfs:range :Sports_Activity ;
                       rdfs:comment "Indicates whether a specific dog breed is suitable for a given sport or activity." ;
                       rdfs:label "isSuitableForActivity" .


###  http://www.semanticweb.org/djem/ontologies/2024/9/DogSportConnect/isTrainedBy
:isTrainedBy rdf:type owl:ObjectProperty ;
             rdfs:domain :Dog ;
             rdfs:range :Trainer ;
             rdfs:comment "Shows the relationship between a dog and its trainer." ;
             rdfs:label "isTrainedBy" .


###  http://www.semanticweb.org/djem/ontologies/2024/9/DogSportConnect/organizedAt
:organizedAt rdf:type owl:ObjectProperty ,
                      owl:FunctionalProperty ,
                      owl:InverseFunctionalProperty ;
             rdfs:domain :Event ;
             rdfs:range :Training_venue ;
             rdfs:comment "Indicates the venue where an event or training session is organized." ;
             rdfs:label "organizedAt" .


###  http://www.semanticweb.org/djem/ontologies/2024/9/DogSportConnect/ownsDog
:ownsDog rdf:type owl:ObjectProperty ,
                  owl:FunctionalProperty ,
                  owl:InverseFunctionalProperty ,
                  owl:AsymmetricProperty ;
         rdfs:domain :Owner ;
         rdfs:range :Dog ;
         rdfs:comment "Represents the ownership relation from an owner's perspective." ;
         rdfs:label "ownsDog" .


###  http://www.semanticweb.org/djem/ontologies/2024/9/DogSportConnect/participatesIn
:participatesIn rdf:type owl:ObjectProperty ;
                rdfs:domain :Dog ;
                rdfs:range :Sports_Activity ;
                owl:propertyChainAxiom ( :ownsDog
                                         :participatesIn
                                       ) ;
                rdfs:comment "Indicates that a dog or person participates in a particular sport or activity." ;
                rdfs:label "participatesIn" .


###  http://www.semanticweb.org/djem/ontologies/2024/9/DogSportConnect/providesTraining
:providesTraining rdf:type owl:ObjectProperty ;
                  rdfs:domain :Trainer ;
                  rdfs:range :Sports_Activity ;
                  rdfs:comment "Shows that a trainer provides training in a specific sport or skill." ;
                  rdfs:label "providesTraining" .


###  http://www.semanticweb.org/djem/ontologies/2024/9/DogSportConnect/supportsActivity
:supportsActivity rdf:type owl:ObjectProperty ;
                  rdfs:domain :Training_venue ;
                  rdfs:range :Sports_Activity ;
                  rdfs:comment "Indicates the support a venue or entity gives to a particular activity." ;
                  rdfs:label "supportsActivity" .


###  http://www.semanticweb.org/djem/ontologies/2024/9/DogSportConnect/trainsAt
:trainsAt rdf:type owl:ObjectProperty ;
          rdfs:domain :Dog ;
          rdfs:range :Training_venue ;
          rdfs:comment "Represents the relationship between a dog and the venue where training occurs." ;
          rdfs:label "trainsAt" .


#################################################################
#    Data properties
#################################################################

###  http://www.semanticweb.org/djem/ontologies/2024/9/DogSportConnect/hasAddress
:hasAddress rdf:type owl:DatatypeProperty ,
                     owl:FunctionalProperty ;
            rdfs:domain :Owner ,
                        :Trainer ;
            rdfs:range xsd:string ;
            rdfs:comment "Specifies the address of the owner or trainer." ,
                         "hasAddress" .


###  http://www.semanticweb.org/djem/ontologies/2024/9/DogSportConnect/hasAge
:hasAge rdf:type owl:DatatypeProperty ;
        rdfs:domain :Dog ,
                    :Owner ,
                    :Trainer ;
        rdfs:range xsd:int ;
        rdfs:comment "Indicates the age of the dog or trainer or owner." ,
                     "hasAge" .


###  http://www.semanticweb.org/djem/ontologies/2024/9/DogSportConnect/hasBreedType
:hasBreedType rdf:type owl:DatatypeProperty ;
              rdfs:domain :Dog ;
              rdfs:range xsd:string ;
              rdfs:comment "Defines the breed type of a dog." ,
                           "hasBreedType" .


###  http://www.semanticweb.org/djem/ontologies/2024/9/DogSportConnect/hasCapacity
:hasCapacity rdf:type owl:DatatypeProperty ;
             rdfs:domain :Training_venue ;
             rdfs:range xsd:integer ;
             rdfs:comment "Specifies the maximum capacity of a training venue." ,
                          "hasCapacity" .


###  http://www.semanticweb.org/djem/ontologies/2024/9/DogSportConnect/hasCertification
:hasCertification rdf:type owl:DatatypeProperty ;
                  rdfs:domain :Trainer ;
                  rdfs:range xsd:boolean ;
                  rdfs:comment "Indicates certifications a trainer holds." ,
                               "hasCertification" .


###  http://www.semanticweb.org/djem/ontologies/2024/9/DogSportConnect/hasContactInfo
:hasContactInfo rdf:type owl:DatatypeProperty ;
                rdfs:domain :Owner ,
                            :Trainer ;
                rdfs:comment "Provides contact information for an owner or trainer." ,
                             "hasContactInfo" .


###  http://www.semanticweb.org/djem/ontologies/2024/9/DogSportConnect/hasDate
:hasDate rdf:type owl:DatatypeProperty ;
         rdfs:domain :Event ;
         rdfs:range xsd:dateTime ;
         rdfs:comment "Specifies the date of an event or training session." ,
                      "hasDate" .


###  http://www.semanticweb.org/djem/ontologies/2024/9/DogSportConnect/hasDuration
:hasDuration rdf:type owl:DatatypeProperty ;
             rdfs:domain :Event ;
             rdfs:range xsd:integer ;
             rdfs:comment "Indicates the duration of a training session or event." ,
                          "hasDuration" .


###  http://www.semanticweb.org/djem/ontologies/2024/9/DogSportConnect/hasEquipment
:hasEquipment rdf:type owl:DatatypeProperty ;
              rdfs:domain :Training_venue ;
              rdfs:comment "Lists the equipment available for a training activity at the Venue" ,
                           "hasEquipment" .


###  http://www.semanticweb.org/djem/ontologies/2024/9/DogSportConnect/hasExperience
:hasExperience rdf:type owl:DatatypeProperty ;
               rdfs:domain :Trainer ;
               rdfs:range xsd:integer ;
               rdfs:comment "Represents the number of years of experience of a trainer." ,
                            "hasExperience" .


###  http://www.semanticweb.org/djem/ontologies/2024/9/DogSportConnect/hasGender
:hasGender rdf:type owl:DatatypeProperty ;
           rdfs:domain :Dog ,
                       :Owner ,
                       :Trainer ;
           rdfs:range xsd:string ;
           rdfs:comment "Indicates the gender of a dog or trainer or owner" ,
                        "hasGender" .


###  http://www.semanticweb.org/djem/ontologies/2024/9/DogSportConnect/hasLocation
:hasLocation rdf:type owl:DatatypeProperty ;
             rdfs:domain :Event ,
                         :Training_venue ;
             rdfs:range xsd:string ;
             rdfs:comment "Provides information about the geographic location of a venue or event." ,
                          "hasLocation" .


###  http://www.semanticweb.org/djem/ontologies/2024/9/DogSportConnect/hasMaxParticipants
:hasMaxParticipants rdf:type owl:DatatypeProperty ;
                    rdfs:domain :Event ;
                    rdfs:range xsd:integer ;
                    rdfs:comment "Defines the maximum number of participants allowed in an event or session." ,
                                 "hasMaxParticipants" .


###  http://www.semanticweb.org/djem/ontologies/2024/9/DogSportConnect/hasName
:hasName rdf:type owl:DatatypeProperty ;
         rdfs:domain :Dog ,
                     :Event ,
                     :Owner ,
                     :Trainer ,
                     :Training_venue ;
         rdfs:range xsd:string ;
         rdfs:comment "Indicates the name of an event, venue, or owner, or trainer, or a dog." ,
                      "hasName" .


###  http://www.semanticweb.org/djem/ontologies/2024/9/DogSportConnect/hasOpeningHours
:hasOpeningHours rdf:type owl:DatatypeProperty ;
                 rdfs:domain :Training_venue ;
                 rdfs:range xsd:dateTime ;
                 rdfs:comment "Specifies the opening hours of a training venue." ,
                              "hasOpeningHours" .


###  http://www.semanticweb.org/djem/ontologies/2024/9/DogSportConnect/hasRating
:hasRating rdf:type owl:DatatypeProperty ;
           rdfs:domain :Trainer ,
                       :Training_venue ;
           rdfs:range xsd:decimal ;
           rdfs:comment "Represents the rating of a trainer or venue." ,
                        "hasRating" .


###  http://www.semanticweb.org/djem/ontologies/2024/9/DogSportConnect/hasRegistrationFee
:hasRegistrationFee rdf:type owl:DatatypeProperty ;
                    rdfs:domain :Event ;
                    rdfs:range xsd:decimal ;
                    rdfs:comment "Indicates the registration fee for participating in an event." ,
                                 "hasRegistrationFee" .


###  http://www.semanticweb.org/djem/ontologies/2024/9/DogSportConnect/hasSpecialization
:hasSpecialization rdf:type owl:DatatypeProperty ;
                   rdfs:domain :Trainer ;
                   rdfs:range xsd:string ;
                   rdfs:comment "Defines the area of specialization of a trainer." ,
                                "hasSpecialization" .


###  http://www.semanticweb.org/djem/ontologies/2024/9/DogSportConnect/hasType
:hasType rdf:type owl:DatatypeProperty ;
         rdfs:domain :Event ,
                     :Training_venue ;
         rdfs:range xsd:string ;
         rdfs:comment "Indicates the type of event, venue." ,
                      "hasType" .


###  http://www.semanticweb.org/djem/ontologies/2024/9/DogSportConnect/hasWeight
:hasWeight rdf:type owl:DatatypeProperty ;
           rdfs:domain :Dog ;
           rdfs:range xsd:decimal ;
           rdfs:comment "Specifies the weight of the dog." ,
                        "hasWeight" .


###  http://www.semanticweb.org/djem/ontologies/2024/9/DogSportConnect/isRecurring
:isRecurring rdf:type owl:DatatypeProperty ;
             rdfs:domain :Event ;
             rdfs:range xsd:boolean ;
             rdfs:comment "isRecurring" ,
                          "ndicates if an event or training session is recurring." .


###  http://www.semanticweb.org/djem/ontologies/2024/9/DogSportConnect/isSuitableForAge
:isSuitableForAge rdf:type owl:DatatypeProperty ;
                  rdfs:subPropertyOf owl:topDataProperty ;
                  rdfs:domain :Sports_Activity ;
                  rdfs:range xsd:integer ;
                  rdfs:comment "Specifies whether an activity is suitable for a particular age range of dogs." ,
                               "isSuitableForAge" .


#################################################################
#    Classes
#################################################################

###  http://www.semanticweb.org/djem/ontologies/2024/9/DogSportConnect#AgilityTrainers
:AgilityTrainers rdf:type owl:Class ;
                 owl:equivalentClass [ owl:intersectionOf ( :Agility
                                                            :Trainer
                                                          ) ;
                                       rdf:type owl:Class
                                     ] ;
                 rdfs:subClassOf :Trainer .


###  http://www.semanticweb.org/djem/ontologies/2024/9/DogSportConnect#BikejoringTrainers
:BikejoringTrainers rdf:type owl:Class ;
                    owl:equivalentClass [ owl:intersectionOf ( :Bikejoring
                                                               :Skijoring
                                                               :Trainer
                                                             ) ;
                                          rdf:type owl:Class
                                        ] ;
                    rdfs:subClassOf :Trainer .


###  http://www.semanticweb.org/djem/ontologies/2024/9/DogSportConnect#CoursingTrainers
:CoursingTrainers rdf:type owl:Class ;
                  owl:equivalentClass [ owl:intersectionOf ( :Lure_Coursing
                                                             :Trainer
                                                           ) ;
                                        rdf:type owl:Class
                                      ] ;
                  rdfs:subClassOf :Trainer .


###  http://www.semanticweb.org/djem/ontologies/2024/9/DogSportConnect#DogFitnessTrainers
:DogFitnessTrainers rdf:type owl:Class ;
                    owl:equivalentClass [ owl:intersectionOf ( :Dog_fitness
                                                               :Trainer
                                                             ) ;
                                          rdf:type owl:Class
                                        ] ;
                    rdfs:subClassOf :Trainer .


###  http://www.semanticweb.org/djem/ontologies/2024/9/DogSportConnect#FlyballTrainers
:FlyballTrainers rdf:type owl:Class ;
                 owl:equivalentClass [ owl:intersectionOf ( :Flyball
                                                            :Trainer
                                                          ) ;
                                       rdf:type owl:Class
                                     ] ;
                 rdfs:subClassOf :Trainer .


###  http://www.semanticweb.org/djem/ontologies/2024/9/DogSportConnect#FrisbeeTrainers
:FrisbeeTrainers rdf:type owl:Class ;
                 owl:equivalentClass [ owl:intersectionOf ( :Frisbee
                                                            :Trainer
                                                          ) ;
                                       rdf:type owl:Class
                                     ] ;
                 rdfs:subClassOf :Trainer .


###  http://www.semanticweb.org/djem/ontologies/2024/9/DogSportConnect#HerdingTrainers
:HerdingTrainers rdf:type owl:Class ;
                 owl:equivalentClass [ owl:intersectionOf ( :Herding
                                                            :Trainer
                                                            :Treibball
                                                          ) ;
                                       rdf:type owl:Class
                                     ] ;
                 rdfs:subClassOf :Trainer .


###  http://www.semanticweb.org/djem/ontologies/2024/9/DogSportConnect#Indoor
:Indoor rdf:type owl:Class ;
        rdfs:subClassOf :Training_venue ;
        rdfs:comment "Indicates that Training Venue is inside of the bilding" ;
        rdfs:label "Indoor" .


###  http://www.semanticweb.org/djem/ontologies/2024/9/DogSportConnect#NoseworkTrainers
:NoseworkTrainers rdf:type owl:Class ;
                  owl:equivalentClass [ owl:intersectionOf ( :Nosework
                                                             :Tracking
                                                             :Trainer
                                                           ) ;
                                        rdf:type owl:Class
                                      ] ;
                  rdfs:subClassOf :Trainer .


###  http://www.semanticweb.org/djem/ontologies/2024/9/DogSportConnect#ObedienceTrainers
:ObedienceTrainers rdf:type owl:Class ;
                   owl:equivalentClass [ owl:intersectionOf ( :Obedience
                                                              :Rally_Obedience
                                                              :Trainer
                                                            ) ;
                                         rdf:type owl:Class
                                       ] ;
                   rdfs:subClassOf :Trainer .


###  http://www.semanticweb.org/djem/ontologies/2024/9/DogSportConnect#OtherTrainers
:OtherTrainers rdf:type owl:Class ;
               owl:equivalentClass [ owl:intersectionOf ( :Canicross
                                                          :Carting
                                                          :Dock_Diving
                                                          :Dog_Parkour
                                                          :Hiking
                                                          :Swimming
                                                          :Trainer
                                                          :Weight_Pulling
                                                        ) ;
                                     rdf:type owl:Class
                                   ] ;
               rdfs:subClassOf :Trainer .


###  http://www.semanticweb.org/djem/ontologies/2024/9/DogSportConnect#Outdoor
:Outdoor rdf:type owl:Class ;
         rdfs:subClassOf :Training_venue ;
         rdfs:comment "Indicates that Training Venue is outside." ;
         rdfs:label "Outdoor" .


###  http://www.semanticweb.org/djem/ontologies/2024/9/DogSportConnect/Agility
:Agility rdf:type owl:Class ;
         rdfs:subClassOf :Sports_Activity ;
         rdfs:comment "Represents a competitive sport where dogs navigate obstacle courses, testing their speed and coordination." ;
         rdfs:label "Agility" .


###  http://www.semanticweb.org/djem/ontologies/2024/9/DogSportConnect/Akita
:Akita rdf:type owl:Class ;
       rdfs:subClassOf :Dog ,
                       [ rdf:type owl:Restriction ;
                         owl:onProperty :isSuitableForActivity ;
                         owl:someValuesFrom :Bikejoring
                       ] ,
                       [ rdf:type owl:Restriction ;
                         owl:onProperty :isSuitableForActivity ;
                         owl:someValuesFrom :Carting
                       ] ,
                       [ rdf:type owl:Restriction ;
                         owl:onProperty :isSuitableForActivity ;
                         owl:someValuesFrom :Dog
                       ] ,
                       [ rdf:type owl:Restriction ;
                         owl:onProperty :isSuitableForActivity ;
                         owl:someValuesFrom :Skijoring
                       ] ,
                       [ rdf:type owl:Restriction ;
                         owl:onProperty :isSuitableForActivity ;
                         owl:someValuesFrom :Weight_Pulling
                       ] ;
       rdfs:comment "A large breed known for its loyalty, originally from Japan, often used as a guard dog." ;
       rdfs:label "Akita" .


###  http://www.semanticweb.org/djem/ontologies/2024/9/DogSportConnect/Alaskan_Malamute
:Alaskan_Malamute rdf:type owl:Class ;
                  rdfs:subClassOf :Dog ,
                                  [ rdf:type owl:Restriction ;
                                    owl:onProperty :isSuitableForActivity ;
                                    owl:someValuesFrom :Bikejoring
                                  ] ,
                                  [ rdf:type owl:Restriction ;
                                    owl:onProperty :isSuitableForActivity ;
                                    owl:someValuesFrom :Canicross
                                  ] ,
                                  [ rdf:type owl:Restriction ;
                                    owl:onProperty :isSuitableForActivity ;
                                    owl:someValuesFrom :Carting
                                  ] ,
                                  [ rdf:type owl:Restriction ;
                                    owl:onProperty :isSuitableForActivity ;
                                    owl:someValuesFrom :Skijoring
                                  ] ,
                                  [ rdf:type owl:Restriction ;
                                    owl:onProperty :isSuitableForActivity ;
                                    owl:someValuesFrom :Weight_Pulling
                                  ] ;
                  rdfs:comment "A strong working breed, ideal for pulling heavy loads, originally bred for Arctic conditions." ;
                  rdfs:label "Alaskan Malamute" .


###  http://www.semanticweb.org/djem/ontologies/2024/9/DogSportConnect/Australian_Shepherd
:Australian_Shepherd rdf:type owl:Class ;
                     rdfs:subClassOf :Dog ,
                                     [ rdf:type owl:Restriction ;
                                       owl:onProperty :isSuitableForActivity ;
                                       owl:someValuesFrom :Agility
                                     ] ,
                                     [ rdf:type owl:Restriction ;
                                       owl:onProperty :isSuitableForActivity ;
                                       owl:someValuesFrom :Dog_fitness
                                     ] ,
                                     [ rdf:type owl:Restriction ;
                                       owl:onProperty :isSuitableForActivity ;
                                       owl:someValuesFrom :Flyball
                                     ] ,
                                     [ rdf:type owl:Restriction ;
                                       owl:onProperty :isSuitableForActivity ;
                                       owl:someValuesFrom :Frisbee
                                     ] ,
                                     [ rdf:type owl:Restriction ;
                                       owl:onProperty :isSuitableForActivity ;
                                       owl:someValuesFrom :Herding
                                     ] ,
                                     [ rdf:type owl:Restriction ;
                                       owl:onProperty :isSuitableForActivity ;
                                       owl:someValuesFrom :Hiking
                                     ] ,
                                     [ rdf:type owl:Restriction ;
                                       owl:onProperty :isSuitableForActivity ;
                                       owl:someValuesFrom :Nosework
                                     ] ,
                                     [ rdf:type owl:Restriction ;
                                       owl:onProperty :isSuitableForActivity ;
                                       owl:someValuesFrom :Obedience
                                     ] ,
                                     [ rdf:type owl:Restriction ;
                                       owl:onProperty :isSuitableForActivity ;
                                       owl:someValuesFrom :Rally_Obedience
                                     ] ,
                                     [ rdf:type owl:Restriction ;
                                       owl:onProperty :isSuitableForActivity ;
                                       owl:someValuesFrom :Treibball
                                     ] ;
                     rdfs:comment "An energetic herding breed known for its intelligence and versatility, commonly used in agility." ;
                     rdfs:label "Australian Shepherd" .


###  http://www.semanticweb.org/djem/ontologies/2024/9/DogSportConnect/Basset_Hound
:Basset_Hound rdf:type owl:Class ;
              rdfs:subClassOf :Dog ;
              rdfs:comment "A scent hound with an excellent sense of smell, often used for hunting small game." ;
              rdfs:label "Basset Hound" .


###  http://www.semanticweb.org/djem/ontologies/2024/9/DogSportConnect/Beagle
:Beagle rdf:type owl:Class ;
        rdfs:subClassOf :Dog ;
        rdfs:comment "A small, friendly breed with strong scenting capabilities, often used for tracking" ;
        rdfs:label "Beagle" .


###  http://www.semanticweb.org/djem/ontologies/2024/9/DogSportConnect/Bernese_Mountain_Dog
:Bernese_Mountain_Dog rdf:type owl:Class ;
                      rdfs:subClassOf :Dog ;
                      rdfs:comment "A large, gentle breed from Switzerland, known for its strength and good nature." ;
                      rdfs:label "Bernese Mountain Dog" .


###  http://www.semanticweb.org/djem/ontologies/2024/9/DogSportConnect/Bichon_Frise
:Bichon_Frise rdf:type owl:Class ;
              rdfs:subClassOf :Dog ;
              rdfs:comment "A small, cheerful companion dog, known for its hypoallergenic coat." ;
              rdfs:label "Bichon Frise" .


###  http://www.semanticweb.org/djem/ontologies/2024/9/DogSportConnect/Bikejoring
:Bikejoring rdf:type owl:Class ;
            rdfs:subClassOf :Sports_Activity ;
            rdfs:comment "Represents a sport involving a dog running alongside a cyclist, pulling them along trails." ;
            rdfs:label "Bikejoring" .


###  http://www.semanticweb.org/djem/ontologies/2024/9/DogSportConnect/Border_Collie
:Border_Collie rdf:type owl:Class ;
               rdfs:subClassOf :Dog ;
               rdfs:comment "A highly intelligent herding breed, renowned for its agility and ability to learn complex tasks." ;
               rdfs:label "Border Collie" .


###  http://www.semanticweb.org/djem/ontologies/2024/9/DogSportConnect/Boston_Terrier
:Boston_Terrier rdf:type owl:Class ;
                rdfs:subClassOf :Dog ;
                rdfs:comment "A small, friendly breed with a tuxedo-like coat, often kept as a companion." ;
                rdfs:label "Boston Terrier" .


###  http://www.semanticweb.org/djem/ontologies/2024/9/DogSportConnect/Boxer
:Boxer rdf:type owl:Class ;
       rdfs:subClassOf :Dog ;
       rdfs:comment "An energetic and playful breed, originally bred for hunting and working roles." ;
       rdfs:label "Boxer" .


###  http://www.semanticweb.org/djem/ontologies/2024/9/DogSportConnect/Bull_Terrier
:Bull_Terrier rdf:type owl:Class ;
              rdfs:subClassOf :Dog ;
              rdfs:comment "A distinctive breed known for its egg-shaped head and playful, loyal demeanor." ;
              rdfs:label "Bull Terrier" .


###  http://www.semanticweb.org/djem/ontologies/2024/9/DogSportConnect/Bulldog
:Bulldog rdf:type owl:Class ;
         rdfs:subClassOf :Dog ;
         rdfs:comment "A muscular breed with a characteristic wrinkled face, known for its calm temperament." ;
         rdfs:label "Bulldog" .


###  http://www.semanticweb.org/djem/ontologies/2024/9/DogSportConnect/Canicross
:Canicross rdf:type owl:Class ;
           rdfs:subClassOf :Sports_Activity ;
           rdfs:comment "Represents cross-country running with dogs, where the owner and dog are attached via a harness." ;
           rdfs:label "Canicross" .


###  http://www.semanticweb.org/djem/ontologies/2024/9/DogSportConnect/Carting
:Carting rdf:type owl:Class ;
         rdfs:subClassOf :Sports_Activity ;
         rdfs:comment "Represents an activity where dogs pull carts, often used by larger breeds." ;
         rdfs:label "Carting" .


###  http://www.semanticweb.org/djem/ontologies/2024/9/DogSportConnect/Cavalier_King_Charles_Spaniel
:Cavalier_King_Charles_Spaniel rdf:type owl:Class ;
                               rdfs:subClassOf :Dog ;
                               rdfs:comment "A friendly toy breed, often used as a lap dog and companion." ;
                               rdfs:label "Cavalier King Charles Spaniel" .


###  http://www.semanticweb.org/djem/ontologies/2024/9/DogSportConnect/Charity_Event
:Charity_Event rdf:type owl:Class ;
               rdfs:subClassOf :Event ;
               rdfs:comment "Represents an event organized to raise funds for a charitable cause related to dogs." ;
               rdfs:label "Charity Event" .


###  http://www.semanticweb.org/djem/ontologies/2024/9/DogSportConnect/Chihuahua
:Chihuahua rdf:type owl:Class ;
           rdfs:subClassOf :Dog ;
           rdfs:comment "The smallest breed, known for its confidence and attachment to owners." ;
           rdfs:label "Chihuahua" .


###  http://www.semanticweb.org/djem/ontologies/2024/9/DogSportConnect/Cocker_Spaniel
:Cocker_Spaniel rdf:type owl:Class ;
                rdfs:subClassOf :Dog ;
                rdfs:comment "A hunting and retrieving breed, known for its long, flowing ears and affectionate nature." ;
                rdfs:label "Cocker Spaniel" .


###  http://www.semanticweb.org/djem/ontologies/2024/9/DogSportConnect/Competition
:Competition rdf:type owl:Class ;
             rdfs:subClassOf :Event ;
             rdfs:comment "Represents a competitive event involving dogs, such as agility or obedience trials." ;
             rdfs:label "Competition" .


###  http://www.semanticweb.org/djem/ontologies/2024/9/DogSportConnect/Dachshund
:Dachshund rdf:type owl:Class ;
           rdfs:subClassOf :Dog ;
           rdfs:comment "small hound breed, originally bred for hunting burrowing animals, known for its elongated body." ;
           rdfs:label "Dachshund" .


###  http://www.semanticweb.org/djem/ontologies/2024/9/DogSportConnect/Dalmatian
:Dalmatian rdf:type owl:Class ;
           rdfs:subClassOf :Dog ;
           rdfs:comment "A distinct spotted breed, often known for its association with firefighting and as a carriage dog." ;
           rdfs:label "Dalmatian" .


###  http://www.semanticweb.org/djem/ontologies/2024/9/DogSportConnect/Doberman_Pinscher
:Doberman_Pinscher rdf:type owl:Class ;
                   rdfs:subClassOf :Dog ;
                   rdfs:comment "A sleek, alert breed, known for its protective instincts and intelligence, often used for guarding." ;
                   rdfs:label "Doberman Pinscher" .


###  http://www.semanticweb.org/djem/ontologies/2024/9/DogSportConnect/Dock_Diving
:Dock_Diving rdf:type owl:Class ;
             rdfs:subClassOf :Sports_Activity ;
             rdfs:comment "Represents a sport where dogs jump off a dock into water, competing for height or distance" ;
             rdfs:label "Dock Diving" .


###  http://www.semanticweb.org/djem/ontologies/2024/9/DogSportConnect/Dog
:Dog rdf:type owl:Class ;
     rdfs:subClassOf [ rdf:type owl:Restriction ;
                       owl:onProperty :hasOwner ;
                       owl:minQualifiedCardinality "1"^^xsd:nonNegativeInteger ;
                       owl:onClass :Owner
                     ] ;
     rdfs:comment "Represents domestic canines of various breeds, owned as pets and trained for activities." ;
     rdfs:label "Dogs" .


###  http://www.semanticweb.org/djem/ontologies/2024/9/DogSportConnect/Dog_Parkour
:Dog_Parkour rdf:type owl:Class ;
             rdfs:subClassOf :Sports_Activity ;
             rdfs:comment "Represents a sport where dogs navigate urban obstacles, improving balance and agility." ;
             rdfs:label "Dog Parkour" .


###  http://www.semanticweb.org/djem/ontologies/2024/9/DogSportConnect/Dog_fitness
:Dog_fitness rdf:type owl:Class ;
             rdfs:subClassOf :Sports_Activity ;
             rdfs:comment "Represents general fitness activities designed to maintain a dog's health and physical condition." ;
             rdfs:label "Dog Fitness" .


###  http://www.semanticweb.org/djem/ontologies/2024/9/DogSportConnect/Event
:Event rdf:type owl:Class ;
       rdfs:subClassOf [ rdf:type owl:Restriction ;
                         owl:onProperty :hosts ;
                         owl:qualifiedCardinality "1"^^xsd:nonNegativeInteger ;
                         owl:onClass :Training_venue
                       ] ;
       rdfs:comment "Represents any organized gathering or activity involving dogs, such as competitions or training sessions.\"" ;
       rdfs:label "Events" .


###  http://www.semanticweb.org/djem/ontologies/2024/9/DogSportConnect/First-Time_Owner
:First-Time_Owner rdf:type owl:Class ;
                  rdfs:subClassOf :Owner ;
                  rdfs:comment "Represents individuals who have recently become dog owners and may require additional guidance and resources" ;
                  rdfs:label "First-Time Owner" .


###  http://www.semanticweb.org/djem/ontologies/2024/9/DogSportConnect/Flyball
:Flyball rdf:type owl:Class ;
         rdfs:subClassOf :Sports_Activity ;
         rdfs:comment "Represents a team relay race for dogs involving hurdles and a ball-fetching mechanism." ;
         rdfs:label "Flyball" .


###  http://www.semanticweb.org/djem/ontologies/2024/9/DogSportConnect/French_Bulldog
:French_Bulldog rdf:type owl:Class ;
                rdfs:subClassOf :Dog ;
                rdfs:comment "A small companion breed, known for its bat-like ears and playful personality." ;
                rdfs:label "French Bulldog" .


###  http://www.semanticweb.org/djem/ontologies/2024/9/DogSportConnect/Frisbee
:Frisbee rdf:type owl:Class ;
         rdfs:subClassOf :Sports_Activity ;
         rdfs:comment "Represents an activity where dogs catch a flying disc, often part of competitive disc dog events." ;
         rdfs:label "Frisbee" .


###  http://www.semanticweb.org/djem/ontologies/2024/9/DogSportConnect/German_Shepherd
:German_Shepherd rdf:type owl:Class ;
                 rdfs:subClassOf :Dog ;
                 rdfs:comment "A versatile working breed, known for its intelligence, often used in police and rescue roles" ;
                 rdfs:label "German Shepherd" .


###  http://www.semanticweb.org/djem/ontologies/2024/9/DogSportConnect/Golden_Retriever
:Golden_Retriever rdf:type owl:Class ;
                  rdfs:subClassOf :Dog ;
                  rdfs:comment "A friendly and intelligent breed, often used for retrieving, assistance, and companionship." ;
                  rdfs:label "Golden Retriever" .


###  http://www.semanticweb.org/djem/ontologies/2024/9/DogSportConnect/Great_Dane
:Great_Dane rdf:type owl:Class ;
            rdfs:subClassOf :Dog ;
            rdfs:comment "One of the largest dog breeds, known for its gentle nature and majestic appearance." ;
            rdfs:label "Great Dane" .


###  http://www.semanticweb.org/djem/ontologies/2024/9/DogSportConnect/Greyhound
:Greyhound rdf:type owl:Class ;
           rdfs:subClassOf :Dog ;
           rdfs:comment "A fast breed, originally bred for hunting by sight, now popular in racing and as a pet.\"" ;
           rdfs:label "Greyhound" .


###  http://www.semanticweb.org/djem/ontologies/2024/9/DogSportConnect/Herding
:Herding rdf:type owl:Class ;
         rdfs:subClassOf :Sports_Activity ;
         rdfs:comment "Represents a working or sporting activity where dogs herd livestock, commonly seen with herding breeds." ;
         rdfs:label "Herding" .


###  http://www.semanticweb.org/djem/ontologies/2024/9/DogSportConnect/Hiking
:Hiking rdf:type owl:Class ;
        rdfs:subClassOf :Sports_Activity ;
        rdfs:comment "Represents long-distance walking with dogs, often on natural trails." ;
        rdfs:label "Hiking" .


###  http://www.semanticweb.org/djem/ontologies/2024/9/DogSportConnect/Irish_Setter
:Irish_Setter rdf:type owl:Class ;
              rdfs:subClassOf :Dog ;
              rdfs:comment "A sporting breed known for its beautiful red coat and energetic personality." ;
              rdfs:label "Irish Setter" .


###  http://www.semanticweb.org/djem/ontologies/2024/9/DogSportConnect/Jack_Russell_Terrier
:Jack_Russell_Terrier rdf:type owl:Class ;
                      rdfs:subClassOf :Dog ;
                      rdfs:comment "A small, energetic hunting breed, often used in agility and earthdog trials." ;
                      rdfs:label "Jack Russell Terrier" .


###  http://www.semanticweb.org/djem/ontologies/2024/9/DogSportConnect/Labrador_Retriever
:Labrador_Retriever rdf:type owl:Class ;
                    rdfs:subClassOf :Dog ;
                    rdfs:comment "A popular breed known for its friendly nature and versatility as a family pet, guide dog, or retriever." ;
                    rdfs:label "Labrador Retriever" .


###  http://www.semanticweb.org/djem/ontologies/2024/9/DogSportConnect/Lure_Coursing
:Lure_Coursing rdf:type owl:Class ;
               rdfs:subClassOf :Sports_Activity ;
               rdfs:comment "Represents a sport where dogs chase a mechanically operated lure, simulating a hunt." ;
               rdfs:label "Lure Coursing" .


###  http://www.semanticweb.org/djem/ontologies/2024/9/DogSportConnect/Maltese
:Maltese rdf:type owl:Class ;
         rdfs:subClassOf :Dog ;
         rdfs:comment "A toy breed, known for its long, silky white coat and affectionate demeanor." ;
         rdfs:label "Maltese" .


###  http://www.semanticweb.org/djem/ontologies/2024/9/DogSportConnect/Meetup
:Meetup rdf:type owl:Class ;
        rdfs:subClassOf :Event ;
        owl:disjointUnionOf ( :Charity_Event
                              :Competition
                              :Meetup
                              :Seminar
                              :Training_Session
                              :Workshop
                            ) ;
        rdfs:comment "Represents a casual gathering of dog owners for socialization or recreational activities." ;
        rdfs:label "Meetup" .


###  http://www.semanticweb.org/djem/ontologies/2024/9/DogSportConnect/Multiple_Dog_Owner
:Multiple_Dog_Owner rdf:type owl:Class ;
                    rdfs:subClassOf :Owner ;
                    rdfs:comment "Represents owners who have more than one dog and may need support for managing a multi-dog household." ;
                    rdfs:label "Multiple Dog Owner" .


###  http://www.semanticweb.org/djem/ontologies/2024/9/DogSportConnect/Newfoundland
:Newfoundland rdf:type owl:Class ;
              rdfs:subClassOf :Dog ;
              rdfs:comment "A large working breed, known for its strength and swimming abilities, often used in water rescue." ;
              rdfs:label "Newfoundland" .


###  http://www.semanticweb.org/djem/ontologies/2024/9/DogSportConnect/Nosework
:Nosework rdf:type owl:Class ;
          rdfs:subClassOf :Sports_Activity ;
          rdfs:comment "Represents an activity where dogs use their sense of smell to locate hidden scents, often used for training or fun." ;
          rdfs:label "Nosework" .


###  http://www.semanticweb.org/djem/ontologies/2024/9/DogSportConnect/Obedience
:Obedience rdf:type owl:Class ;
           rdfs:subClassOf :Sports_Activity ;
           rdfs:comment "Represents a competitive sport that tests a dog's ability to follow commands accurately." ;
           rdfs:label "Obedience" .


###  http://www.semanticweb.org/djem/ontologies/2024/9/DogSportConnect/Owner
:Owner rdf:type owl:Class ;
       rdfs:subClassOf [ rdf:type owl:Restriction ;
                         owl:onProperty :ownsDog ;
                         owl:minQualifiedCardinality "1"^^xsd:nonNegativeInteger ;
                         owl:onClass :Dog
                       ] ;
       rdfs:comment "Represents individuals who own one or more dogs, responsible for their care and participation in activities." ;
       rdfs:label "Owners" .


###  http://www.semanticweb.org/djem/ontologies/2024/9/DogSportConnect/Pembroke_Welsh_Corgi
:Pembroke_Welsh_Corgi rdf:type owl:Class ;
                      rdfs:subClassOf :Dog ;
                      rdfs:comment "A herding breed, known for its short legs and friendly demeanor, originally bred for cattle herding." ;
                      rdfs:label "Pembroke Welsh Corgi" .


###  http://www.semanticweb.org/djem/ontologies/2024/9/DogSportConnect/Pomeranian
:Pomeranian rdf:type owl:Class ;
            rdfs:subClassOf :Dog ;
            rdfs:comment "A small companion breed, known for its fluffy coat and outgoing personality." ;
            rdfs:label "Pomeranian" .


###  http://www.semanticweb.org/djem/ontologies/2024/9/DogSportConnect/Poodle
:Poodle rdf:type owl:Class ;
        rdfs:subClassOf :Dog ;
        rdfs:comment "A highly intelligent breed that comes in multiple sizes, known for its hypoallergenic coat.\"" ;
        rdfs:label "Poodle" .


###  http://www.semanticweb.org/djem/ontologies/2024/9/DogSportConnect/Professional_Trainer_Owner
:Professional_Trainer_Owner rdf:type owl:Class ;
                            rdfs:subClassOf :Owner ;
                            rdfs:comment "Represents owners who are also professional dog trainers, with advanced training skills." ;
                            rdfs:label "Professional Trainer Owner" .


###  http://www.semanticweb.org/djem/ontologies/2024/9/DogSportConnect/Pug
:Pug rdf:type owl:Class ;
     rdfs:subClassOf :Dog ;
     rdfs:comment "A small breed with a wrinkled face and curled tail, known for its friendly and playful nature." ;
     rdfs:label "Pug" .


###  http://www.semanticweb.org/djem/ontologies/2024/9/DogSportConnect/Rally_Obedience
:Rally_Obedience rdf:type owl:Class ;
                 rdfs:subClassOf :Sports_Activity ;
                 rdfs:comment "Represents a sport combining traditional obedience commands with a sequence of activities." ;
                 rdfs:label "Rally Obedience" .


###  http://www.semanticweb.org/djem/ontologies/2024/9/DogSportConnect/Reactive_Dog_Owner
:Reactive_Dog_Owner rdf:type owl:Class ;
                    rdfs:subClassOf :Owner ;
                    rdfs:comment "Represents owners of dogs that exhibit reactive behaviors and may need specialized training or support." ;
                    rdfs:label "Reactive Dog Owner" .


###  http://www.semanticweb.org/djem/ontologies/2024/9/DogSportConnect/Rottweiler
:Rottweiler rdf:type owl:Class ;
            rdfs:subClassOf :Dog ;
            rdfs:comment "A strong working breed, originally used for herding and guarding, known for its loyalty." ;
            rdfs:label "Rottweiler" .


###  http://www.semanticweb.org/djem/ontologies/2024/9/DogSportConnect/Saint_Bernard
:Saint_Bernard rdf:type owl:Class ;
               rdfs:subClassOf :Dog ;
               rdfs:comment "A large breed, originally bred for rescue work in the Alps, known for its gentle nature." ;
               rdfs:label "Saint Bernard" .


###  http://www.semanticweb.org/djem/ontologies/2024/9/DogSportConnect/Samoyed
:Samoyed rdf:type owl:Class ;
         rdfs:subClassOf :Dog ;
         rdfs:comment "A fluffy white working breed, originally bred for herding and sledding, known for its friendly demeanor." ;
         rdfs:label "Samoyed" .


###  http://www.semanticweb.org/djem/ontologies/2024/9/DogSportConnect/Seminar
:Seminar rdf:type owl:Class ;
         rdfs:subClassOf :Event ;
         rdfs:comment "Represents an educational event where participants can learn more about dog training, health, or behavior." ;
         rdfs:label "Seminar" .


###  http://www.semanticweb.org/djem/ontologies/2024/9/DogSportConnect/Shiba_Inu
:Shiba_Inu rdf:type owl:Class ;
           rdfs:subClassOf :Dog ;
           rdfs:comment "A small, agile breed from Japan, known for its fox-like appearance and independence." ;
           rdfs:label "Shiba Inu" .


###  http://www.semanticweb.org/djem/ontologies/2024/9/DogSportConnect/Shih_Tzu
:Shih_Tzu rdf:type owl:Class ;
          rdfs:subClassOf :Dog ;
          rdfs:comment "A small breed, originally bred as a companion for Chinese royalty, known for its long flowing coat." ;
          rdfs:label "Shih Tzu" .


###  http://www.semanticweb.org/djem/ontologies/2024/9/DogSportConnect/Siberian_Husky
:Siberian_Husky rdf:type owl:Class ;
                rdfs:subClassOf :Dog ;
                rdfs:comment "A medium-sized working breed, known for its endurance and strength, often used for sledding." ;
                rdfs:label "Siberian Husky" .


###  http://www.semanticweb.org/djem/ontologies/2024/9/DogSportConnect/Skijoring
:Skijoring rdf:type owl:Class ;
           rdfs:subClassOf :Sports_Activity ;
           rdfs:comment "Represents a winter sport where a dog pulls a person on skis, requiring strength and coordination." ;
           rdfs:label "Skijoring" .


###  http://www.semanticweb.org/djem/ontologies/2024/9/DogSportConnect/Special_Needs_Dog_Owner
:Special_Needs_Dog_Owner rdf:type owl:Class ;
                         rdfs:subClassOf :Owner ;
                         rdfs:comment "Represents owners of dogs with special needs, such as health conditions or disabilities." ;
                         rdfs:label "Special Needs Dog Owner" .


###  http://www.semanticweb.org/djem/ontologies/2024/9/DogSportConnect/Sports_Activity
:Sports_Activity rdf:type owl:Class ;
                 rdfs:comment "Represents different types of sports and activities in which dogs can participate, such as agility or frisbee." ;
                 rdfs:label "Sports Activities" .


###  http://www.semanticweb.org/djem/ontologies/2024/9/DogSportConnect/Sports_Enthusiast_Owner
:Sports_Enthusiast_Owner rdf:type owl:Class ;
                         rdfs:subClassOf :Owner ;
                         rdfs:comment "Represents owners who are actively involved in canine sports and enjoy training their dogs for such activities." ;
                         rdfs:label "Sports Enthusiast Owner" .


###  http://www.semanticweb.org/djem/ontologies/2024/9/DogSportConnect/Swimming
:Swimming rdf:type owl:Class ;
          rdfs:subClassOf :Sports_Activity ;
          rdfs:comment "Represents a physical activity where dogs swim, used for exercise or rehabilitation." ;
          rdfs:label "Swimming" .


###  http://www.semanticweb.org/djem/ontologies/2024/9/DogSportConnect/Tracking
:Tracking rdf:type owl:Class ;
          rdfs:subClassOf :Sports_Activity ;
          rdfs:comment "Represents an activity where dogs follow a scent trail, often used in search and rescue." ;
          rdfs:label "Tracking" .


###  http://www.semanticweb.org/djem/ontologies/2024/9/DogSportConnect/Trainer
:Trainer rdf:type owl:Class ;
         rdfs:subClassOf [ rdf:type owl:Restriction ;
                           owl:onProperty :hasExperience ;
                           owl:minQualifiedCardinality "1"^^xsd:nonNegativeInteger ;
                           owl:onDataRange xsd:int
                         ] ;
         rdfs:comment "Represents individuals who provide professional training services to dogs, helping them develop specific skills" ;
         rdfs:label "Trainers" .


###  http://www.semanticweb.org/djem/ontologies/2024/9/DogSportConnect/Training_Session
:Training_Session rdf:type owl:Class ;
                  rdfs:subClassOf :Event ;
                  rdfs:comment "Represents a scheduled time for structured training activities with dogs." ;
                  rdfs:label "Training Session" .


###  http://www.semanticweb.org/djem/ontologies/2024/9/DogSportConnect/Training_venue
:Training_venue rdf:type owl:Class ;
                owl:disjointUnionOf ( :Indoor
                                      :Outdoor
                                    ) ;
                rdfs:comment "Represents physical locations where dogs are trained or participate in activities, such as indoor centers or outdoor fields." ;
                rdfs:label "Training Venues" .


###  http://www.semanticweb.org/djem/ontologies/2024/9/DogSportConnect/Treibball
:Treibball rdf:type owl:Class ;
           rdfs:subClassOf :Sports_Activity ;
           rdfs:comment "Represents a sport where dogs push large balls into a goal, simulating herding behavior." ;
           rdfs:label "Treibball" .


###  http://www.semanticweb.org/djem/ontologies/2024/9/DogSportConnect/Vizsla
:Vizsla rdf:type owl:Class ;
        rdfs:subClassOf :Dog ;
        rdfs:comment "A medium-sized hunting breed, known for its affectionate nature and strong bond with its owner." ;
        rdfs:label "Vizsla" .


###  http://www.semanticweb.org/djem/ontologies/2024/9/DogSportConnect/Weight_Pulling
:Weight_Pulling rdf:type owl:Class ;
                rdfs:subClassOf :Sports_Activity ;
                rdfs:comment "Represents a strength-based sport where dogs pull weighted carts, testing their power." ;
                rdfs:label "Weight Pulling" .


###  http://www.semanticweb.org/djem/ontologies/2024/9/DogSportConnect/Weimaraner
:Weimaraner rdf:type owl:Class ;
            rdfs:subClassOf :Dog ;
            rdfs:comment "A medium-to-large hunting breed, known for its sleek silver coat, originally bred in Germany for hunting large game." ;
            rdfs:label "Weimaraner" .


###  http://www.semanticweb.org/djem/ontologies/2024/9/DogSportConnect/Workshop
:Workshop rdf:type owl:Class ;
          rdfs:subClassOf :Event ;
          rdfs:comment "Represents a hands-on event aimed at teaching specific skills related to dogs." ;
          rdfs:label "Workshop" .


###  http://www.semanticweb.org/djem/ontologies/2024/9/DogSportConnect/half-breed
:half-breed rdf:type owl:Class ;
            rdfs:subClassOf :Dog ;
            rdfs:comment "Mixed-breed dogs that combine characteristics of two or more pure breeds." ;
            rdfs:label "Half-breed" .


###  Generated by the OWL API (version 4.5.29.2024-05-13T12:11:03Z) https://github.com/owlcs/owlapi
